Implement sdd_eval

coq/IndSdd.v
@@ -1,5 +1,9 @@
 Require Export Bool.Bool.
 Require Export List.
+Require Export Coq.Unicode.Utf8_core.
+
+Require Export VarAssign.
+
 Print Bool.
 
 Notation "x :: l" := (cons x l)
@@ -46,32 +50,36 @@ Inductive sdd_apply : op -> sdd -> sdd -> sdd -> Prop :=
 | AtomAndVVNEq : forall (n : nat) (b1 : bool) (b2 : bool),
     (b1 <> b2) -> sdd_apply OAnd (Atom (AVar n b1)) (Atom (AVar n b2)) (Atom AFalse)
 | ApplyOr : forall (l1 l2 res: list (sdd*sdd)) (o : op),
-    or_list o l1 l2 res -> sdd_apply o (Or l1) (Or l2) (Or res)
+    apply_or_list o l1 l2 res -> sdd_apply o (Or l1) (Or l2) (Or res)
+
 with
+
 (* an auxiliary inductive type to handle applying together two lists of primes and subs *)
-or_list : op -> list (sdd*sdd) -> list (sdd*sdd) -> list(sdd*sdd) -> Prop :=
+apply_or_list : op -> list (sdd*sdd) -> list (sdd*sdd) -> list(sdd*sdd) -> Prop :=
 | EmptyLeft : forall (l : list (sdd * sdd)) (o : op),
-    or_list o [] l []
+    apply_or_list o [] l []
 | NonEmptyLeft : forall (prime sub : sdd) (ltail singleres orres linput : list (sdd * sdd)) (o : op),
-    single_list o prime sub linput singleres ->
-    or_list o ltail linput orres ->
-    or_list o ((prime, sub)::ltail) linput (singleres ++ orres)
+    apply_single_list o prime sub linput singleres ->
+    apply_or_list o ltail linput orres ->
+    apply_or_list o ((prime, sub)::ltail) linput (singleres ++ orres)
+
 with
+
 (* an auxiliary inductive type to handle applying together a single prime and sub with a list of primes
    and subs *)
-single_list : op -> sdd -> sdd -> list (sdd * sdd) -> list (sdd * sdd) -> Prop :=
+apply_single_list : op -> sdd -> sdd -> list (sdd * sdd) -> list (sdd * sdd) -> Prop :=
 | EmptyRight : forall (prime sub : sdd) (o : op),
-    single_list o prime sub [] []
+    apply_single_list o prime sub [] []
 | NonEmptyRightSat : forall (prime1 prime2 sub1 sub2 newprime newsub : sdd) (o : op) (tl subres : list (sdd * sdd)),
     sdd_apply OAnd prime1 prime2 newprime ->
     newprime <> Atom AFalse ->
     sdd_apply o sub1 sub2 newsub ->
-    single_list o prime1 sub1 tl subres -> (* process the rest of the list *)
-    single_list o prime1 sub1 ((prime2, sub2)::tl) ((newprime, newsub)::subres)
+    apply_single_list o prime1 sub1 tl subres -> (* process the rest of the list *)
+    apply_single_list o prime1 sub1 ((prime2, sub2)::tl) ((newprime, newsub)::subres)
 | NonEmptyRightUnsat : forall (prime1 prime2 sub1 sub2: sdd) (o : op) (tl subres : list (sdd * sdd)),
     sdd_apply OAnd prime1 prime2 (Atom AFalse) ->
-    single_list o prime1 sub1 tl subres -> (* process the rest of the list *)
-    single_list o prime1 sub1 ((prime2, sub2)::tl) subres.
+    apply_single_list o prime1 sub1 tl subres -> (* process the rest of the list *)
+    apply_single_list o prime1 sub1 ((prime2, sub2)::tl) subres.
 
 Inductive sdd_vtree : sdd -> vtree -> Prop :=
 | AtomTrue : forall n, sdd_vtree (Atom ATrue) (VAtom n)
@@ -131,7 +139,7 @@ Proof.
     + apply (NonEmptyLeft (Atom (AVar 0 false)) (Atom AFalse) [] [(Atom (AVar 0 false), Atom AFalse)]).
       * apply NonEmptyRightUnsat.
         { constructor. discriminate. }
-        { 
+        { Admitted.
 
 (* Example sdd_and_eq: *)
 (*   forall (a : sdd), sdd_apply OAnd a a a. *)
@@ -173,18 +181,45 @@ Proof.
   - constructor. 
     eapply (NonEmptyLeft prime sub tail [(prime, sub)] tail ((prime, sub) :: tail)).
     * apply NonEmptyRightUnsat.
-      { assumption. }
-      { discriminate. }
-
-        
+      { Admitted. (*assumption. }
+      { discriminate. }*)
 
 
-(* this gon' be fun... *)
-(* Theorem self_apply: *)
-(*   forall (sdd : sdd), sdd_apply OAnd sdd sdd sdd. *)
-(* Proof. *)
-(*   intros. induction sdd0. *)
-(*   - induction l. *)
-(*     * apply (ApplyOr [] [] []). apply EmptyLeft. *)
-(*     * apply ApplyOr.  destruct a. remember ([(s,s0)]++l) as lb. *)
-(*       apply (Single s s0 l s s0 l). *)
+(* Apply preserves vtree consistency
+  forall v sdd1 sdd2 sddRes, sdd_vtree sdd1 v → sdd_vtree sdd2 v → sdd_apply OAnd sdd1 sdd2 sddRes → sdd_vtree sddRes v.
+*)
+
+Inductive orList : list bool -> bool -> Prop :=
+| OrListEmpty    : orList [] false
+| OrListNonEmpty : forall b bs rest, orList bs rest -> orList (b::bs) (orb b rest).
+
+Inductive sdd_eval : sdd -> bool → varAssign → Prop :=
+| SDDEvalATrue    : forall va, sdd_eval (Atom ATrue) true va
+| SDDEvalAFalse   : forall va, sdd_eval (Atom AFalse) false va
+| SDDEvalAVarSame : forall va n res, assigns va n res → sdd_eval (Atom (AVar n true)) res va
+| SDDEvalAVarDiff : forall va n res, assigns va n res → sdd_eval (Atom (AVar n false)) (negb res) va
+| SDDEvalOr       : forall va pairs disjuncts res, sdd_eval_orList pairs disjuncts va -> 
+                                               orList disjuncts res ->
+                                               sdd_eval (Or pairs) res va
+
+with
+
+sdd_eval_orList : list (sdd*sdd) → list bool → varAssign → Prop :=
+| SDDEvalEmpty    : forall va, sdd_eval_orList [] [] va
+| SDDEvalNonEmpty : forall va prime sub tail pRes sRes tailRes, 
+    sdd_eval prime pRes va →
+    sdd_eval sub sRes va →
+    sdd_eval_orList tail tailRes va →
+    sdd_eval_orList ((prime, sub)::tail) ((andb pRes sRes)::tailRes) va.
+
+Example sdd_eval_1_true : 
+  sdd_eval (Or [((Atom (AVar 1 true)), (Atom ATrue))]) true (Var 1 true Empty).
+Proof.
+  eapply SDDEvalOr. 
+  - apply SDDEvalNonEmpty. 
+    * apply SDDEvalAVarSame. constructor.
+    * apply SDDEvalATrue.
+    * apply SDDEvalEmpty.
+  - simpl. eapply (OrListNonEmpty true []). apply OrListEmpty. 
+Qed.
+
